Semantics/IRStepThms.thy
@@ -12,130 +12,11 @@ transition to the same subsequent configuration. Therefore, our step semantics
 is deterministic.
 \<close>
 
-(*
-definition stepping_nodes :: "(IRNode \<Rightarrow> bool) set" where
-  "stepping_nodes = {
-    is_sequential_node,
-    is_IfNode,
-    is_AbstractEndNode,
-    is_NewInstanceNode,
-    is_LoadFieldNode,
-    is_SignedDivNode,
-    is_SignedRemNode,
-    is_LoadFieldNode,
-    is_StoreFieldNode
-  }"
-
-inductive_cases StepE[elim!]:\<^marker>\<open>tag invisible\<close>
-  "g, p \<turnstile> (nid,m,h) \<rightarrow> next"
-
-lemma stepping_nodes_distinct:
-  assumes "sel \<in> stepping_nodes \<and> sel node"
-  shows "\<forall> oth \<in> stepping_nodes - {sel} . \<not>(oth node)"
-  using assms unfolding stepping_nodes_def sorry
-
-
-proof (induction arbitrary: m h rule: step.induct)
-  case (SequentialNode nid nid')
-  have "is_sequential_node \<in> stepping_nodes" unfolding stepping_nodes_def by simp
-  then have distinct: "\<forall> oth \<in> stepping_nodes - {is_sequential_node} . \<not>(oth (kind g nid))"
-    using stepping_nodes_distinct SequentialNode(1) by auto
-  obtain next' where "g, p \<turnstile> (nid, m, h) \<rightarrow> next'"
-    using SequentialNode.hyps(1) step.SequentialNode
-    by blast
-  then have "next' = (nid', m, h)"
-    apply (induct rule: step.induct) using SequentialNode sorry
-  show ?case apply (rule allI) (*using step.cases*) apply (induction rule: step.induct)
-    using distinct unfolding stepping_nodes_def
-    using is_IfNode_def is_NewInstanceNode_def is_LoadFieldNode_def is_SignedDivNode_def is_SignedRemNode_def
-    is_LoadFieldNode_def is_StoreFieldNode_def 
-    apply (rule stepping_nodes_distinct [where sel = is_sequential_node, where node = "kind g nid"])
-  then show ?case apply (rule stepping_nodes_distinct [where sel = is_sequential_node, where node = "kind g nid"])?
-next
-  case (IfNode nid cond tb fb condE m val nid' h)
-  then show ?case sorry
-next
-  case (EndNodes nid merge i phis inps inpsE m vs m' h)
-  then show ?case sorry
-next
-  case (NewInstanceNode nid f obj nid' h' ref h m' m)
-  then show ?case sorry
-next
-  case (LoadFieldNode nid f obj nid' objE m ref h v m')
-  then show ?case sorry
-next
-  case (SignedDivNode nid x y zero sb nxt xe ye m v1 v2 v m' h)
-  then show ?case sorry
-next
-  case (SignedRemNode nid x y zero sb nxt xe ye m v1 v2 v m' h)
-  then show ?case sorry
-next
-  case (StaticLoadFieldNode nid f nid' h v m' m)
-  then show ?case sorry
-next
-  case (StoreFieldNode nid f newval uu obj nid' newvalE objE m val ref h' h m')
-  then show ?case sorry
-next
-  case (StaticStoreFieldNode nid f newval uv nid' newvalE m val h' h m')
-  then show ?case sorry
-qed
-*)
-
 subsubsection \<open>Control-flow Step is Deterministic\<close>
 
 inductive_cases StepE[elim]:\<^marker>\<open>tag invisible\<close>
   "g, p \<turnstile> state \<rightarrow> val"
 
-(*
-definition xor :: "bool \<Rightarrow> bool \<Rightarrow> bool"    (infixl "[+]" 60)
-  where "A [+] B \<equiv> (A \<and> \<not> B) \<or> (\<not> A \<and> B)"
-
-lemma xor_false [simp]:
-  "A [+] False = A"
-  by (simp add: xor_def)
-
-(*lemma xor_true [simp]:
-  "(A [+] B [+] True) = ((A [+] True) \<and> (\<not>B))"
-  by (simp add: xor_def)*)
-
-lemma xor_resolve_true [simp]:
-  "False [+] True = True"
-  by (simp add: xor_def)
-
-lemma xor_unfold [simp]:
-  "A [+] (B [+] C) = A [+] B [+] C"
-  using xor_def by force
-
-definition control_nodes :: "(IRNode \<Rightarrow> bool) list" where
-  "control_nodes = 
-    [is_sequential_node,
-    is_FixedGuardNode,
-    is_BytecodeExceptionNode,
-    is_IfNode,
-    is_AbstractEndNode,
-    is_NewArrayNode,
-    is_ArrayLengthNode,
-    is_LoadIndexedNode,
-    is_StoreIndexedNode,
-    is_NewInstanceNode,
-    is_SignedDivNode,
-    is_SignedRemNode,
-    is_LoadFieldNode,
-    is_StoreFieldNode]"
-
-definition is_control_flow :: "IRNode \<Rightarrow> bool" where
-  "is_control_flow node = fold (\<or>) (map (\<lambda>f. f node) control_nodes) False"
-
-definition control_flow_exclusive :: "IRNode \<Rightarrow> bool" where
-  "control_flow_exclusive node = fold ([+]) (map (\<lambda>f. f node) control_nodes) False"
-
-
-lemma exclusive_control:
-  "is_control_flow n \<Longrightarrow> control_flow_exclusive n"
-  unfolding is_control_flow_def control_flow_exclusive_def
-  control_nodes_def apply simp
-  by (cases n; simp)
-*)
 
 theorem stepDet':
    "(g, p \<turnstile> state \<rightarrow> next) \<Longrightarrow>
@@ -151,7 +32,7 @@ proof (induction arbitrary: next' rule: "step.induct")
     apply (metis (no_types, lifting) Pair_inject is_AbstractEndNode.simps)
     by force+
 next
-  case (FixedGuardNode nid cond before "next" condE m val nid' h)
+  case (FixedGuardNode nid cond before "next" m val nid' h)
   then show ?case apply (elim StepE)
     by force+
 next
@@ -159,88 +40,89 @@ next
   then show ?case apply (elim StepE)
     by force+
 next
-  case (IfNode nid cond tb fb condE m val nid' h)
+  case (IfNode nid cond tb fb m val nid' h)
   then show ?case apply (elim StepE)
     apply force+
     \<comment> \<open>IfNode rule uses expression evaluation\<close>
-    using evalDet repDet apply fastforce
+    using graphDet apply fastforce
     by force+
 next
-  case (EndNodes nid merge i phis inps inpsE m vs m' h)
+  case (EndNodes nid merge i phis inps m vs m' h)
   have notseq: "\<not>(is_sequential_node (kind g nid))"
     using EndNodes
     by (metis is_AbstractEndNode.simps is_EndNode.elims(2) is_LoopEndNode_def is_sequential_node.simps(18) is_sequential_node.simps(36))
   from EndNodes show ?case apply (elim StepE)
     using notseq apply force
                   apply force apply force apply force
-    using indexof_det 
+    using indexof_det
     unfolding is_AbstractEndNode.simps
     is_AbstractMergeNode.simps any_usage.simps usages.simps inputs.simps ids_def
-    sorry
+               apply (smt (verit, del_insts) Collect_cong encodeEvalAllDet ids_def ids_some old.prod.inject)
+    by force+
 next
-  case (NewArrayNode nid len st nid' lenE m length' arrayType h' ref h refNo h'' m')
+  case (NewArrayNode nid len st nid' m length' arrayType h' ref h refNo h'' m')
   then show ?case apply (elim StepE) apply force+
   \<comment> \<open>NewArrayNode rule uses expression evaluation\<close>
-  using evalDet repDet apply fastforce
+  using graphDet apply fastforce
   by force+
 next
-  case (ArrayLengthNode nid x nid' xE m ref h arrayVal length' m')
+  case (ArrayLengthNode nid x nid' m ref h arrayVal length' m')
   then show ?case apply (elim StepE) apply force+
   \<comment> \<open>ArrayLengthNode rule uses expression evaluation\<close>
-  using evalDet repDet apply fastforce
+  using graphDet apply fastforce
   by force+
 next             
-  case (LoadIndexedNode nid index guard array nid' indexE m indexVal arrayE ref h arrayVal loaded m')
+  case (LoadIndexedNode nid index guard array nid'  m indexVal ref h arrayVal loaded m')
   then show ?case apply (elim StepE) apply force+
   \<comment> \<open>LoadIndexedNode rule uses expression evaluation\<close>
-  using evalDet repDet
+  using graphDet
   apply (metis IRNode.inject(28) Pair_inject Value.inject(2))
   by force+
 next
-  case (StoreIndexedNode nid check val st index guard array nid' indexE m indexVal arrayE ref valE "value" h arrayVal updated h' m')
+  case (StoreIndexedNode nid check val st index guard array nid' m indexVal ref "value" h arrayVal updated h' m')
   then show ?case apply (elim StepE) apply force+
   \<comment> \<open>StoreIndexedNode rule uses expression evaluation\<close>
-    using evalDet repDet
+    using graphDet
     apply (metis IRNode.inject(55) Pair_inject Value.inject(2))
   by force+
 next
   case (NewInstanceNode nid cname obj nid' h' ref h m' m)
   then show ?case apply (elim StepE) by force+
 next
-  case (LoadFieldNode nid f obj nid' objE m ref h v m')
+  case (LoadFieldNode nid f obj nid' m ref h v m')
   then show ?case apply (elim StepE) apply force+
   \<comment> \<open>LoadFieldNode rule uses expression evaluation\<close>
-    using evalDet repDet apply fastforce
+    using graphDet apply fastforce
   by force+
 next
-  case (SignedDivNode nid x y zero sb nxt xe ye m v1 v2 v m' h)
+  case (SignedDivNode nid x y zero sb nxt m v1 v2 v m' h)
   then show ?case apply (elim StepE) apply force+
   \<comment> \<open>SignedDivNode rule uses expression evaluation\<close>
-    using evalDet repDet
+    using graphDet
     apply (metis IRNode.inject(49) Pair_inject)
   by force+
 next
-  case (SignedRemNode nid x y zero sb nxt xe ye m v1 v2 v m' h)
+  case (SignedRemNode nid x y zero sb nxt m v1 v2 v m' h)
   then show ?case apply (elim StepE) apply force+
   \<comment> \<open>SignedRemNode rule uses expression evaluation\<close>
-    using evalDet repDet
+    using graphDet
     apply (metis IRNode.inject(52) Pair_inject)
   by force+
 next
   case (StaticLoadFieldNode nid f nid' h v m' m)
   then show ?case apply (elim StepE) by force+
 next
-  case (StoreFieldNode nid f newval uu obj nid' newvalE objE m val ref h' h m')
+  case (StoreFieldNode nid f newval uu obj nid' m val ref h' h m')
   then show ?case apply (elim StepE) apply force+
   \<comment> \<open>StoreFieldNode rule uses expression evaluation\<close>
-    using evalDet repDet
+    using graphDet
     apply (metis IRNode.inject(54) Pair_inject Value.inject(2) option.inject)
   by force+
 next
-  case (StaticStoreFieldNode nid f newval uv nid' newvalE m val h' h m')
+  case (StaticStoreFieldNode nid f newval uv nid' m val h' h m')
   then show ?case apply (elim StepE) apply force+
   \<comment> \<open>StaticStoreFieldNode rule uses expression evaluation\<close>
-    using evalDet repDet by fastforce
+    using graphDet by fastforce
 qed
 
 theorem stepDet:
@@ -258,7 +140,7 @@ lemma IfNodeStepCases:
   assumes "[m, p] \<turnstile> condE \<mapsto> v"
   assumes "g, p \<turnstile> (nid, m, h) \<rightarrow> (nid', m, h)"
   shows "nid' \<in> {tb, fb}"
-  by (metis insert_iff old.prod.inject step.IfNode stepDet assms)
+  by (metis insert_iff old.prod.inject step.IfNode stepDet assms encodeeval.simps)
 
 lemma IfNodeSeq:
   shows "kind g nid = IfNode cond tb fb \<longrightarrow> \<not>(is_sequential_node (kind g nid))"
@@ -268,7 +150,7 @@ lemma IfNodeCond:
   assumes "kind g nid = IfNode cond tb fb"
   assumes "g, p \<turnstile> (nid, m, h) \<rightarrow> (nid', m, h)"
   shows "\<exists> condE v. ((g \<turnstile> cond \<simeq> condE) \<and> ([m, p] \<turnstile> condE \<mapsto> v))"
-  using assms(2,1) by (induct "(nid,m,h)" "(nid',m,h)" rule: step.induct; auto)
+  using assms(2,1) encodeeval.simps by (induct "(nid,m,h)" "(nid',m,h)" rule: step.induct; auto)
 
 lemma step_in_ids:
   assumes "g, p \<turnstile> (nid, m, h) \<rightarrow> (nid', m', h')"
